---
{"dg-publish":true,"permalink":"/10-19-teaching/14-algebra-qual/problem-bank/pool-problems/group-theory/preimage-of-a-subgroup/","tags":["group_theory"],"updated":"2025-03-14T15:28:37-07:00"}
---

Suppose $\phi:G\to G'$ is a surjective homomorphism, $H\leq G$ is a subgroup containing $\ker(\phi)$, and $H'=\phi(H)$. Prove $\phi^{-1}(H')=H$, where $\phi^{-1}(H')=\{g\in G\,\mid\, \phi(g)\in H'\}$. Make sure to state explicitly where each hypothesis is used.

> [!info]- View $\LaTeX$ code
> ```
> Suppose $\phi:G\to G'$ is a surjective homomorphism, $H\leq G$ is a subgroup containing $\ker(\phi)$, and $H'=\phi(H)$. Prove $\phi^{-1}(H')=H$, where $\phi^{-1}(H')=\{g\in G\,\mid\, \phi(g)\in H'\}$. Make sure to state explicitly where each hypothesis is used.
> ```